Duplicate: big progress on step_simulation, only Ijumptbl left

backend/Duplicateaux.ml
@@ -1,4 +1,4 @@
 open RTL
 open Maps
 
-let duplicate_aux f = ((fn_code f), PTree.empty)
+let duplicate_aux f = (((fn_code f), (fn_entrypoint f)), PTree.empty)
